Sestoft proven correct (that was fast!)

Launchbury/SestoftCorrect.thy
@@ -1,5 +1,5 @@
 theory SestoftCorrect
-imports Sestoft Launchbury
+imports Sestoft Launchbury BalancedTraces
 begin
 
 
@@ -59,111 +59,44 @@ next
 case (Let as \<Gamma> L body \<Delta> z S)
   from Let(1) Let(4)
   have "atom ` domA as \<sharp>* (\<Gamma>, S)" by (simp add: fresh_star_Pair)
-  hence "(\<Gamma>, Let as body, S) \<Rightarrow> (as@\<Gamma>, body, S)"..
+  hence "(\<Gamma>, Terms.Let as body, S) \<Rightarrow> (as@\<Gamma>, body, S)"..
   also have "\<dots> \<Rightarrow>\<^sup>* (\<Delta>, z, S)" by (rule Let) fact
   finally show ?case.
 qed
 
 type_synonym trace = "conf list"
 
-(*
-inductive trace :: "conf \<Rightarrow> trace \<Rightarrow> conf \<Rightarrow> bool"  where
-  trace_nil[iff]: "trace conf [] conf"
-| trace_cons[intro]: "trace conf' T end \<Longrightarrow> conf \<Rightarrow> conf' \<Longrightarrow> trace conf (conf'#T) end"
-
-lemma build_trace:
-  "c \<Rightarrow>\<^sup>* c' \<Longrightarrow> \<exists> T. trace c T c'"
-proof(induction rule: converse_rtranclp_induct)
-  have "trace c' [] c'"..
-  thus "\<exists>T. trace c' T c'"..
-next
-  fix y z
-  assume "y \<Rightarrow> z"
-  assume "\<exists>T. trace z T c'"
-  then obtain T where "trace z T c'"..
-  with `y \<Rightarrow> z`
-  have "trace y (z#T) c'" by auto
-  thus "\<exists>T. trace y T c'" by blast
-qed
-
-lemma destruct_trace:  "trace c T c' \<Longrightarrow> c \<Rightarrow>\<^sup>* c'"
-  by (induction rule:trace.induct) auto
-
-definition extends :: "stack \<Rightarrow> stack \<Rightarrow> bool" (infix "\<lesssim>" 50) where
-  "S \<lesssim> S' = (\<exists> S''. S' = S'' @ S)"
-
 fun stack :: "conf \<Rightarrow> stack" where "stack (\<Gamma>, e, S) = S"
 
-fun bal :: "conf \<Rightarrow> trace \<Rightarrow> conf \<Rightarrow> bool" where
-  "bal c T c' = (trace c T c' \<and> (list_all (\<lambda>c'. stack c \<lesssim> stack c') T \<and> stack c' = stack c))"
-lemma bal_consE:
-  assumes "bal c\<^sub>1 (c\<^sub>2 # T) c\<^sub>5"
-  assumes "length (stack c\<^sub>2)
-  obtains T\<^sub>1 
+interpretation traces step.
 
-*)
+interpretation balance_trace step  stack
+  apply default
+  apply (erule step.cases)
+  apply auto
+  done
 
-
-
-(*
-lemma bal_trace[case_names empty app var "let"]:
+lemma lambda_stop:
+  assumes "isLam e"
   assumes "bal (\<Gamma>, e, S) T (\<Delta>, z, S)"
-  obtains
-    "T = []" and "\<Delta> = \<Gamma>" and "z = e"
-  | x f y e' T\<^sub>1 T\<^sub>2
-   where "e = App f x"
-    and "bal (\<Gamma>, e, Arg x # S) T\<^sub>1 (\<Delta>, Lam [y]. e', Arg x # S)"
-    and "bal (\<Delta>, e'[y::=x], S) T\<^sub>2 c'"
-    and "T = (\<Gamma>, e, Arg x # S) # T\<^sub>1 @  (\<Delta>, e'[y::=x], S) # T\<^sub>2"
-  | \<Gamma> x S  \<Delta> y e' T\<^sub>1 T\<^sub>2
-   where "c = (\<Gamma>, Var x, S)"
-    and "map_of \<Gamma> x = Some e"
-    and "bal (delete x \<Gamma>, e, Upd x # S) T\<^sub>1 (\<Delta>, z, Upd x # S)"
-    and "bal ((x,z)#\<Delta>, z, S) T\<^sub>2 c'"
-    and "T = (delete x \<Gamma>, e, Upd x # S) # T\<^sub>1 @ ((x,z)#\<Delta>, z, S) # T\<^sub>2"
-  | \<Gamma> as e' S T\<^sub>1
-   where "c = (\<Gamma>, Let as e', S)"
-    and "atom ` domA as \<sharp>* \<Gamma>"
-    and "atom ` domA as \<sharp>* S"
-    and "bal (as @ \<Gamma>, e', S) T\<^sub>1 c'"
-    and "T = (as @ \<Gamma>, e', S) # T\<^sub>1"
-sorry
-
-
-lemma lemma_3:
-  assumes "bal (\<Gamma>, e, S) T (\<Delta>, z, S)"
-  assumes "isLam z"
-  shows "\<Gamma> : e \<Down>\<^bsub>L\<^esub> \<Delta> : z"
-thm measure_induct_rule
-using assms
-proof(induction T arbitrary: \<Gamma> e S \<Delta> z rule: measure_induct_rule[where f = length])
-  case (less T \<Gamma> e S \<Delta> z)
-  from `bal (\<Gamma>, e, S) T (\<Delta>, z, S)`
-  show ?case
-  proof(induction rule: bal_trace)
-  case empty
-    from `isLam z` obtain y e' where "z = Lam [y]. e'" by (cases z rule:isLam.cases) auto
-    with empty show ?case by (auto intro: reds.intros)
-  next 
-  case (app \<Gamma> x e S \<Delta> y e' T\<^sub>1 T\<^sub>2)
-    from `T = (\<Gamma>, e, Arg x # S) # T\<^sub>1 @ (\<Delta>, e'[y::=x], S) # T\<^sub>2`
-    have l1: "length T\<^sub>1 < length T" and l2: "length T\<^sub>2 < length T" by auto
-    note IH1 = less(1)[OF l1 app(2) isLam_Lam]
-    note IH2 = less(1)[OF _ app(3)]
-*)  
-    
-      
-
+  shows "T=[]"
+  using assms
+  apply -
+  apply (erule balE)
+  apply (erule trace.cases)
+  apply (auto elim: step.cases)
+  done
+  
 lemma lemma_3:
   assumes "bal (\<Gamma>, e, S) T (\<Delta>, z, S)"
   assumes "isLam z"
   shows "\<Gamma> : e \<Down>\<^bsub>flattn S\<^esub> \<Delta> : z"
-thm measure_induct_rule
 using assms
 proof(induction T arbitrary: \<Gamma> e S \<Delta> z rule: measure_induct_rule[where f = length])
   case (less T \<Gamma> e S \<Delta> z)
   from `bal (\<Gamma>, e, S) T (\<Delta>, z, S)`
   have "trace (\<Gamma>, e, S) T (\<Delta>, z, S)" and "list_all (\<lambda>c'. S \<lesssim> stack c') T" unfolding bal.simps by auto
+
   from this(1)
   show ?case
   proof(cases)
@@ -177,28 +110,73 @@ proof(induction T arbitrary: \<Gamma> e S \<Delta> z rule: measure_induct_rule[w
     from `(\<Gamma>, e, S) \<Rightarrow> conf'`
     show ?thesis
     proof(cases)
-      case (app\<^sub>1 e x)
+    case (app\<^sub>1 e x)
+      obtain T\<^sub>1 c\<^sub>3 c\<^sub>4 T\<^sub>2
+      where "T' = T\<^sub>1 @ c\<^sub>4 # T\<^sub>2" and prem1: "bal (\<Gamma>, e, Arg x # S) T\<^sub>1 c\<^sub>3" and "c\<^sub>3 \<Rightarrow> c\<^sub>4" and prem2: "bal c\<^sub>4 T\<^sub>2 (\<Delta>, z, S)"
+        by (rule bal_consE[OF  `bal _ T _`[unfolded app\<^sub>1 trace_cons]]) (simp, rule)
+
+      from `T = _` `T' = _` have "length T\<^sub>1 < length T" and "length T\<^sub>2 < length T" by auto
+
+      from prem1 have "stack c\<^sub>3 =  Arg x # S" by (auto dest:  bal_stackD)
+      moreover
+      from prem2 have "stack c\<^sub>4 = S" by (auto dest: bal_stackD)
+      moreover
+      note `c\<^sub>3 \<Rightarrow> c\<^sub>4`
+      ultimately
+      obtain \<Delta>' y e' where "c\<^sub>3 = (\<Delta>', Lam [y]. e', Arg x # S)" and "c\<^sub>4 = (\<Delta>', e'[y ::= x], S)"
+        by (auto elim!: step.cases simp del: exp_assn.eq_iff)
       
-      show ?thesis sorry
+      from less(1)[OF `length T\<^sub>1 < length T` prem1[unfolded `c\<^sub>3 = _` `c\<^sub>4 = _`] isLam_Lam]
+      have "\<Gamma> : e \<Down>\<^bsub>x # (flattn S)\<^esub> \<Delta>' : Lam [y]. e'" by simp
+      moreover
+      from less(1)[OF `length T\<^sub>2 < length T` prem2[unfolded `c\<^sub>3 = _` `c\<^sub>4 = _`] `isLam z`]
+      have "\<Delta>' : e'[y::=x] \<Down>\<^bsub>flattn S\<^esub> \<Delta> : z" by simp
+      ultimately
+      show ?thesis unfolding app\<^sub>1
+        by (rule reds_ApplicationI)
     next
-      case (app\<^sub>2 y e x S')
+    case (app\<^sub>2 y e x S')
       from `conf' =_` `S = _ # S'` `S \<lesssim> stack conf'`
       have False by (auto simp add: extends_def)
       thus ?thesis..
     next
-      case (var\<^sub>1 x e)
-      show ?thesis sorry
+    case (var\<^sub>1 x e)
+      obtain T\<^sub>1 c\<^sub>3 c\<^sub>4 T\<^sub>2
+      where "T' = T\<^sub>1 @ c\<^sub>4 # T\<^sub>2" and prem1: "bal (delete x \<Gamma>, e, Upd x # S) T\<^sub>1 c\<^sub>3" and "c\<^sub>3 \<Rightarrow> c\<^sub>4" and prem2: "bal c\<^sub>4 T\<^sub>2 (\<Delta>, z, S)"
+        by (rule bal_consE[OF  `bal _ T _`[unfolded var\<^sub>1 trace_cons]]) (simp, rule)
+      
+      from `T = _` `T' = _` have "length T\<^sub>1 < length T" and "length T\<^sub>2 < length T" by auto
+
+
+      from prem1 have "stack c\<^sub>3 = Upd x # S" by (auto dest:  bal_stackD)
+      moreover
+      from prem2 have "stack c\<^sub>4 = S" by (auto dest: bal_stackD)
+      moreover
+      note `c\<^sub>3 \<Rightarrow> c\<^sub>4`
+      ultimately
+      obtain \<Delta>' z' where "c\<^sub>3 = (\<Delta>', z', Upd x # S)" and "c\<^sub>4 = ((x,z')#\<Delta>', z', S)" and "isLam z'"
+        by (auto elim!: step.cases simp del: exp_assn.eq_iff)
+
+      from `isLam z'` and prem2[unfolded `c\<^sub>4 = _`]
+      have "T\<^sub>2 = []" by (rule lambda_stop)
+      with prem2 `c\<^sub>4 = _`
+      have "z' = z" and "\<Delta> = (x,z)#\<Delta>'" by auto
+          
+      from less(1)[OF `length T\<^sub>1 < length T` prem1[unfolded `c\<^sub>3 = _` `c\<^sub>4 = _`  `z' = _`] `isLam z`]
+      have "delete x \<Gamma> : e \<Down>\<^bsub>x # flattn S\<^esub> \<Delta>' : z" by simp
+      with `map_of _ _ = _`
+      show ?thesis unfolding var\<^sub>1(1) `\<Delta> = _` by rule
     next
-      case (var\<^sub>2 x S')
+    case (var\<^sub>2 x S')
       from `conf' = _` `S = _ # S'` `S \<lesssim> stack conf'`
       have False by (auto simp add: extends_def)
       thus ?thesis..
     next
-      case (let\<^sub>1 as e)
+    case (let\<^sub>1 as e)
       from `T = conf' # T'` have "length T' < length T" by auto
       moreover
       have "bal (as @ \<Gamma>, e, S) T' (\<Delta>, z, S)" 
-        using trace_cons `conf' = _`  `list_all _ _`  by simp
+        using trace_cons `conf' = _`  `list_all _ _` by auto
       moreover
       note `isLam z`
       ultimately
